rocq-osiris/theories/program_logic/pure/expr_rules.v
@@ -900,21 +900,6 @@ Proof.
   eapply pure_ret; last reflexivity. encode.
 Qed.
 
-Lemma pure_eval_EOpPhysEq_cont η e1 e2 (x1 x2 : cont) :
-  pure (eval η e1) (singleton x1) ⊥ ->
-  pure (eval η e2) (singleton x2) ⊥ ->
-  (* Representability hypotheses last for [x1] and [x2] evar initialisation *)
-  representable x1.(address) ->
-  representable x2.(address) ->
-  pure (eval η (EOpPhysEq e1 e2)) (λ b, b = locations.eqb x1 x2) ⊥.
-Proof.
-  intros He1 He2 Hx1 Hx2. simpl_eval.
-  eapply pure_bind. instantiate (1:= λ '(a1, a2), singleton x1 a1 ∧ singleton x2 a2).
-  { eapply pure_par; eauto. }
-  intros [??] [-> ->].
-  eapply pure_ret; last reflexivity. encode.
-Qed.
-
 (* EOpEq (e1 e2 : expr) *)
 
 Lemma pure_eval_EOpEq η e1 e2 (x1 x2 : Z) :
